Start cleaning up chan specs+proof before relying on it in other proofs

new/proof/github_com/goose_lang/goose/model/channel/logatom/chan_au_base.v
@@ -6,20 +6,16 @@ From iris.algebra Require Import auth gset.
 Require Export New.code.github_com.goose_lang.goose.model.channel.
 From New.generatedproof.github_com.goose_lang.goose Require Import model.channel.
 
-(* NOTE: must shadow iris ghost_var *)
-From Perennial.algebra Require Import ghost_var.
-
-(** The mathematical model of channel states. This represents the logical
-    behavior of channels independent of the implementation details. *)
+(** The specification state for a channel. *)
 Module chan_rep.
 Inductive t (V : Type) : Type :=
-| Buffered (buff: list V)     (* Buffered channel with pending messages *)
+| Buffered (buff : list V)     (* Buffered channel with pending messages *)
 | Idle                        (* Empty unbuffered channel, ready for operations *)
-| SndPending (v: V)          (* Unbuffered channel with sender waiting *)
+| SndPending (v : V)          (* Unbuffered channel with sender waiting *)
 | RcvPending                 (* Unbuffered channel with receiver waiting *)
-| SndCommit (v: V)           (* Sender committed, waiting for receiver to complete *)
+| SndCommit (v : V)           (* Sender committed, waiting for receiver to complete *)
 | RcvCommit                  (* Receiver committed, waiting for sender to complete *)
-| Closed (drain: list V)  (* Closed channel, possibly drain remaining messages *)
+| Closed (drain : list V)  (* Closed channel, possibly drain remaining messages *)
 .
 #[global] Instance witness V : Inhabited (t V) := populate!.
 
@@ -38,13 +34,13 @@ End chan_rep.
     in that we don't go to the SndWait state logically until an offer
     is about to be accepted. *)
 Inductive chan_phys_state (V : Type) : Type :=
-| Buffered (buffer: list V)     (* Channel with buffered messages *)
+| Buffered (buffer : list V)     (* Channel with buffered messages *)
 | Idle                        (* Ready for operations *)
 | SndWait (v : V)            (* Sender offers *)
 | RcvWait                    (* Receiver offers *)
 | SndDone (v : V)            (* Sender operation completed, handshake in progress *)
 | RcvDone            (* Receiver operation completed, handshake in progress *)
-| Closed (buffer: list V)  (* Closed channel *)
+| Closed (buffer : list V)  (* Closed channel *)
 .
 
 Global Arguments Idle {V}.
@@ -78,13 +74,14 @@ Record chan_names := {
   chan_cap : w64;                        (* The channel capacity *)
 }.
 
-(** Type class for ghost state associated with channels *)
 Class chanG Σ V := ChanG {
   offerG :: ghost_varG Σ (chan_rep.t V);
   offer_lockG :: ghost_varG Σ (option (offer_lock V));
   offer_parked_propG :: savedPropG Σ;
   offer_parked_predG :: savedPredG Σ (V * bool);
 }.
+Global Hint Mode chanG - + : typeclass_instances.
+Local Hint Mode chanG - - : typeclass_instances.
 
 Definition chanΣ V : gFunctors :=
   #[ ghost_varΣ (chan_rep.t V); ghost_varΣ (option (offer_lock V));
@@ -94,28 +91,18 @@ Definition chanΣ V : gFunctors :=
   subG (chanΣ V) Σ → chanG Σ V.
 Proof. solve_inG. Qed.
 
-Section base.
+Section defns.
 Context `{hG: heapGS Σ, !ffi_semantics _ _}.
 Context {sem_fn : GoSemanticsFunctions} {pre_sem : go.PreSemantics}
   {sem : go.ChanSemantics}.
 Local Set Default Proof Using "sem_fn pre_sem sem".
 
-Context `{!chanG Σ V}.
+Context (ch : loc) (γ : chan_names) (V : Type) `{!chanG Σ V}.
 Context `{!ZeroVal V} `{!TypedPointsto V} `{!IntoValTyped V t}.
-
-(* Remove the later from a saved prop if we have later credits. *)
-Lemma saved_prop_lc_agree γ dq1 dq2 P Q :
-   £ 1 -∗ saved_prop_own γ dq1 P -∗ saved_prop_own γ dq2 Q -∗ |={⊤}=> (P ≡ Q).
-Proof.
-  iIntros "Hlc HP HQ".
-  iDestruct (saved_prop_agree with "HP HQ") as "Heq".
-  iMod (lc_fupd_elim_later with "Hlc Heq") as "H3".
-  iModIntro. done.
-Qed.
 
 (** Maps physical channel states to their heap representations.
     Each state corresponds to specific field values in the Go struct. *)
-Definition chan_phys (ch: loc) (s: chan_phys_state V) : iProp Σ :=
+Definition chan_phys (s: chan_phys_state V) : iProp Σ :=
   match s with
     | Closed [] =>
         (∃ (slice_val: slice.t),
@@ -173,192 +160,15 @@ Definition chan_phys (ch: loc) (s: chan_phys_state V) : iProp Σ :=
     end.
 
 (** Bundles together offer-related ghost state for atomic operations *)
-Definition saved_offer (γ : chan_names) (q : Qp)
+Definition saved_offer (q : Qp)
   (lock_val : option (offer_lock V))
   (parked_prop continuation_prop : iProp Σ) : iProp Σ :=
-  ghost_var γ.(offer_lock_name) (DfracOwn q) lock_val ∗
+  ghost_var γ.(offer_lock_name) q lock_val ∗
   saved_prop_own γ.(offer_parked_prop_name) (DfracOwn q) parked_prop ∗
   saved_prop_own γ.(offer_continuation_name) (DfracOwn q) continuation_prop.
 
-Notation offer_bundle_full γ := (saved_offer γ 1%Qp).
-Notation offer_bundle_half γ := (saved_offer γ (1/2)%Qp).
-
-Definition offer_bundle_empty (γ : chan_names) : iProp Σ :=
-  offer_bundle_full γ None True True.
-
-Lemma offer_idle_to_send γ v parked_prop cont :
-  offer_bundle_empty γ ==∗
-  offer_bundle_half γ (Some (Snd v)) parked_prop cont ∗
-  offer_bundle_half γ (Some (Snd v)) parked_prop cont.
-Proof.
-  iIntros "[Hlock [Hoffer Hcont]]".
-  iMod (ghost_var_update (Some (Snd v)) with "Hlock") as "[Hlock1 Hlock2]".
-  iMod (saved_prop_update cont with "Hcont") as "[Hcont1 Hcont2]".
-  iMod (saved_prop_update parked_prop with "Hoffer") as "[Hoffer1 Hoffer2]".
-  iModIntro. iFrame.
-Qed.
-
-Lemma offer_halves_to_idle γ x y parked_prop cont :
-  offer_bundle_half γ (Some x) parked_prop cont -∗
-   offer_bundle_half γ (Some y) parked_prop cont ==∗
-  offer_bundle_empty γ.
-Proof.
-  iIntros "[Hlock [Hoffer Hcont]]".
-  iIntros "[Hlock2 [Hoffer2 Hcont2]]".
-  iCombine "Hlock Hlock2" gives %Heq.
-  assert (x = y) by (destruct_and!; congruence); subst.
-  iCombine "Hlock Hlock2" as "Hlock".
-  iMod (saved_prop_update_halves True with "Hoffer Hoffer2") as "[Hoffer Hoffer2]".
-  iMod (saved_prop_update_halves True with "Hcont Hcont2") as "[Hcont Hcont2]".
-  iCombine "Hcont Hcont2" as "Hcont".
-  iCombine "Hoffer Hoffer2" as "Hoffer".
-  iMod (ghost_var_update None with "Hlock") as "Hlock".
-  iModIntro. unfold offer_bundle_empty. unfold offer_bundle_full. iFrame.
-  unfold saved_prop_own.
-  rewrite dfrac_op_own.
-  rewrite Qp.half_half.
-  iFrame.
-Qed.
-
-Lemma offer_idle_to_recv γ parked_prop cont:
-  offer_bundle_empty γ ==∗
-  offer_bundle_half γ (Some Rcv) parked_prop cont ∗
-  offer_bundle_half γ (Some Rcv) parked_prop cont.
-Proof.
-   iIntros "[Hlock [Hoffer Hcont]]".
-  iMod (ghost_var_update (Some (Rcv)) with "Hlock") as "[Hlock1 Hlock2]".
-  iMod (saved_prop_update cont with "Hcont") as "[Hcont1 Hcont2]".
-  iMod (saved_prop_update parked_prop with "Hoffer") as "[Hoffer1 Hoffer2]".
-  iModIntro. iFrame.
-Qed.
-
-Lemma offer_reset γ :
-  ∀ parked_prop cont state,
-   offer_bundle_full γ state parked_prop cont ==∗
-  offer_bundle_empty γ.
-Proof.
-  intros parked_prop cont state.
-  iIntros "[Hlock [Hoffer Hcont]]".
-  iMod (ghost_var_update None with "Hlock") as "Hlock".
-  iMod (saved_prop_update True with "Hcont") as "Hcont".
-  iMod (saved_prop_update True with "Hoffer") as "Hoffer".
-  iModIntro.
-  iFrame.
-Qed.
-
-Lemma offer_bundle_agree γ q1 q2
-  lock1 parked1 cont1 lock2 parked2 cont2 :
-  saved_offer γ q1 lock1 parked1 cont1 ∗
-  saved_offer γ q2 lock2 parked2 cont2 ⊢
-  ⌜lock1 = lock2⌝ ∗
-  ▷(parked1 ≡ parked2) ∗ ▷(cont1 ≡ cont2).
-Proof.
-  iIntros "[[Hl1 [Hp1 Hc1]] [Hl2 [Hp2 Hc2]]]".
-  iDestruct (ghost_var_agree with "Hl1 Hl2") as %->.
-  iDestruct (saved_prop_agree with "Hp1 Hp2") as "Hp_eq".
-  iDestruct (saved_prop_agree with "Hc1 Hc2") as "Hc_eq".
-  auto.
-Qed.
-
-Lemma offer_bundle_lc_agree γ
-  lock1 parked1 cont1 lock2 parked2 cont2 :
-  £ 1 -∗
-  saved_offer γ (1/2) lock1 parked1 cont1 -∗
-  saved_offer γ (1/2) lock2 parked2 cont2 -∗
-  |={⊤}=> ⌜lock1 = lock2⌝ ∗
-         (parked1 ≡ parked2) ∗ (cont1 ≡ cont2) ∗
-         offer_bundle_empty γ.
-Proof.
-  iIntros "Hlc1".
-  iIntros "[Hl1 [Hp1 Hc1]]".
-  iIntros "[Hl2 [Hp2 Hc2]]".
-  iDestruct (ghost_var_agree with "[$Hl1] [$Hl2]") as %->.
-  iDestruct (saved_prop_agree with "[$Hp1] [$Hp2]") as "#Hp_eq".
-  iDestruct (saved_prop_agree with "[$Hc1] [$Hc2]") as "#Hc_eq".
-
-  iCombine "Hp_eq Hc_eq" as "Heq".
-  iClear "Hp_eq Hc_eq".
-  iMod (lc_fupd_elim_later with "Hlc1 Heq") as "[Hp_eq Hc_eq]".
-  unfold offer_bundle_empty. unfold offer_bundle_full.
-  iFrame.
-  iSplitR; first done.  (* ⌜lock2 = lock2⌝ is trivial *)
-
-  (* Combine and update ghost variable *)
-  iCombine "Hl1 Hl2" as "Hlock".
-  iMod ((ghost_var_update None) with "Hlock") as "Hlock".
-
-  (* Update saved propositions using halves lemmas *)
-  iMod (saved_prop_update_halves True with "Hp1 Hp2") as "[Hp1 Hp2]".
-  iMod (saved_prop_update_halves True with "Hc1 Hc2") as "[Hc1 Hc2]".
-
-  (* Combine the updated halves to get full ownership *)
-  iCombine "Hp1 Hp2" as "Hparked".
-  iCombine "Hc1 Hc2" as "Hcont".
-
-  (* Simplify the combined fractions *)
-  rewrite dfrac_op_own Qp.half_half.
-
-  iFrame.
-  auto.
-Qed.
-
-Lemma saved_offer_fractional_invalid γ q1 q2 lock1 parked1 cont1 lock2 parked2 cont2 :
-  (1 < q1 + q2)%Qp →
-  saved_offer γ q1 lock1 parked1 cont1 -∗
-  saved_offer γ q2 lock2 parked2 cont2 -∗
-  False.
-Proof.
-  iIntros (Hq) "[Hlock1 [Hp1 Hc1]] [Hlock2 [Hp2 Hc2]]".
-  iDestruct (ghost_var_valid_2 with "Hlock1 Hlock2") as "[%Hvalid _]".
-  iPureIntro.
-apply Qp.lt_nge in Hq.
-contradiction.
-Qed.
-
-Lemma saved_offer_half_full_invalid γ lock1 parked1 cont1 lock2 parked2 cont2 :
-  saved_offer γ (1/2) lock1 parked1 cont1 -∗
-  saved_offer γ 1 lock2 parked2 cont2 -∗
-  False.
-Proof.
-  iApply saved_offer_fractional_invalid.
-  compute_done. (* 1/2 + 1 = 3/2 > 1 *)
-Qed.
-
-Definition chan_rep (γ : gname) (q : Qp) (s : chan_rep.t V) : iProp Σ :=
-  ghost_var γ (DfracOwn q) s.
-
-Notation chan_rep_full γ s := (chan_rep γ 1 s).
-Notation chan_rep_half γ s := (chan_rep γ (1/2)%Qp s).
-Notation chan_rep_auth γ s := (chan_rep_half γ s).
-Notation chan_rep_frag γ s := (chan_rep_half γ s).
-
-Lemma chan_rep_update γ s s' :
-  chan_rep_full γ s ==∗ chan_rep_full γ s'.
-Proof.
-  iApply (ghost_var_update s' γ s).
-Qed.
-
-Lemma chan_rep_agree γ q1 q2 s s' :
-  chan_rep γ q1 s -∗ chan_rep γ q2 s' -∗ ⌜s = s'⌝.
-Proof.
-  iIntros "H1 H2". by iApply (ghost_var_agree with "H1 H2").
-Qed.
-
-(* NOTE: unused *)
-#[local] Lemma chan_rep_combine γ s s' :
-  chan_rep_half γ s -∗ chan_rep_half γ s' -∗ chan_rep_full γ s.
-Proof.
-  iIntros "H1 H2". iDestruct (chan_rep_agree with "H1 H2") as %->.
-  iCombine "H1 H2" as "H". done.
-Qed.
-
-Lemma chan_rep_halves_update γ s1 s2 s' :
-  chan_rep_half γ s1 -∗ chan_rep_half γ s2 ==∗
-     chan_rep_half γ s' ∗ chan_rep_half γ s'.
-Proof.
-  rewrite /chan_rep.
-  apply ghost_var_update_halves.
-Qed.
+Definition chan_rep (q : Qp) (s : chan_rep.t V) : iProp Σ :=
+  ghost_var γ.(state_name) q s.
 
 Definition chan_cap_valid (s : chan_rep.t V) (cap : Z) : Prop :=
   match s with
@@ -376,205 +186,146 @@ Definition chan_cap_valid (s : chan_rep.t V) (cap : Z) : Prop :=
 
 (** ** Channel Ownership Predicate *)
 
-(* chan_cap is directly user accessible *)
-
 (** Represents ownership of a channel with its logical state *)
-Definition own_chan (ch: loc) (s: chan_rep.t V) (γ: chan_names) : iProp Σ :=
-  "Hchanrepfrag" ∷ chan_rep_half γ.(state_name) s ∗
+Definition own_chan (s: chan_rep.t V) : iProp Σ :=
+  "Hchanrepfrag" ∷ chan_rep (1/2) s ∗
   "%Hcapvalid" ∷ ⌜ chan_cap_valid s (sint.Z $ chan_cap γ) ⌝.
 
-Lemma own_chan_agree ch s s' γ :
-   own_chan ch s γ -∗ own_chan ch s' γ -∗ ⌜s = s'⌝.
-Proof.
-  iIntros "H1 H2". iNamedSuffix "H1" "1". iNamedSuffix "H2" "2".
-  iDestruct (ghost_var_agree with "[$Hchanrepfrag1] [$Hchanrepfrag2]") as "%Hag".
-  unfold chan_cap_valid in *.
-  by iApply (ghost_var_agree with "Hchanrepfrag1 Hchanrepfrag2").
-Qed.
-
-(* Needs [chan_cap_valid s'' cap] as precondition? *)
-Lemma own_chan_halves_update s'' ch s s' γ :
-  chan_cap_valid s'' (sint.Z $ chan_cap γ) →
-  own_chan ch s γ -∗ own_chan ch s' γ ==∗
-  own_chan ch s'' γ ∗ own_chan ch s'' γ.
-Proof.
-  intros Hvalid.
-  iIntros "(Hv1 & %) (Hv2 & %)". rewrite /named.
-  iMod (chan_rep_halves_update with "Hv1 Hv2") as "[$ $]".
-  iFrame "#∗".
-  iPureIntro.
-  auto.
-Qed.
-
-Lemma own_chan_buffer_size ch γ buf :
-  own_chan ch (chan_rep.Buffered buf) γ -∗
-  ⌜Z.of_nat (length buf) ≤ sint.Z $ chan_cap γ⌝.
-Proof.
-  iNamed 1.
-  simpl in Hcapvalid.
-  iPureIntro. lia.
-Qed.
-
-Lemma own_chan_drain_size ch γ drain :
-  own_chan ch (chan_rep.Closed drain) γ -∗
-  ⌜Z.of_nat (length drain) ≤ sint.Z $ chan_cap γ⌝.
-Proof.
-  iNamed 1.
-  simpl in Hcapvalid.
-  destruct drain.
-  { simpl. iPureIntro; lia. }
-  iPureIntro. lia.
-Qed.
-
-(** uncurry *)
-Definition K (Φ : V → bool → iProp Σ) : (V * bool) → iProp Σ :=
-  λ '(v,b), Φ v b.
-
 (** Inner atomic update for receive completion (second phase of handshake) *)
-Definition recv_nested_au ch (γ: chan_names) (Φ : V → bool → iProp Σ) : iProp Σ :=
+Definition recv_nested_au (Φ : V → bool → iProp Σ) : iProp Σ :=
    |={⊤,∅}=>
-    ▷∃ s, "Hocinner" ∷ own_chan ch s γ ∗
+    ▷∃ s, "Hocinner" ∷ own_chan s ∗
      "Hcontinner" ∷
     (match s with
     (* Case: Sender has committed, complete the exchange *)
-    | chan_rep.SndCommit v => own_chan ch chan_rep.Idle γ ={∅,⊤}=∗ Φ v true
+    | chan_rep.SndCommit v => own_chan chan_rep.Idle ={∅,⊤}=∗ Φ v true
     (* Case: Channel is closed with no messages *)
-    | chan_rep.Closed [] => own_chan ch s γ ={∅,⊤}=∗ Φ (zero_val V) false
+    | chan_rep.Closed [] => own_chan s ={∅,⊤}=∗ Φ (zero_val V) false
     | _ => True
     end).
 
 (** Slow path receive: may need to block and wait *)
-Definition recv_au ch (γ: chan_names) (Φ : V → bool → iProp Σ) : iProp Σ :=
+Definition recv_au (Φ : V → bool → iProp Σ) : iProp Σ :=
    |={⊤,∅}=>
-    ▷∃ s, "Hoc" ∷ own_chan ch s γ ∗
+    ▷∃ s, "Hoc" ∷ own_chan s ∗
      "Hcont" ∷
     (match s with
     (* Case: Sender is waiting, can complete immediately *)
     | chan_rep.SndPending v =>
-          own_chan ch chan_rep.RcvCommit γ ={∅,⊤}=∗ Φ v true
+          own_chan chan_rep.RcvCommit ={∅,⊤}=∗ Φ v true
     (* Case: Channel is idle, need to wait for sender *)
     | chan_rep.Idle =>
-          own_chan ch (chan_rep.RcvPending) γ ={∅,⊤}=∗
-              recv_nested_au ch γ Φ
+          own_chan (chan_rep.RcvPending) ={∅,⊤}=∗
+              recv_nested_au Φ
     (* Case: Channel is closed *)
-    | chan_rep.Closed [] => own_chan ch s γ ={∅,⊤}=∗ Φ (zero_val V) false
+    | chan_rep.Closed [] => own_chan s ={∅,⊤}=∗ Φ (zero_val V) false
     (* Case: Closed but still have values to drain *)
-    | chan_rep.Closed (v::rest) => (own_chan ch (chan_rep.Closed rest) γ ={∅,⊤}=∗ Φ v true)
+    | chan_rep.Closed (v::rest) => (own_chan (chan_rep.Closed rest) ={∅,⊤}=∗ Φ v true)
     (* Case: Buffered channel with values in buffer *)
-    | chan_rep.Buffered (v::rest) => (own_chan ch (chan_rep.Buffered rest) γ ={∅,⊤}=∗ Φ v true)
+    | chan_rep.Buffered (v::rest) => (own_chan (chan_rep.Buffered rest) ={∅,⊤}=∗ Φ v true)
     | _ => True
     end).
 
 (** Fast path receive: immediate completion when possible *)
-Definition nonblocking_recv_au ch γ (Φ : V → bool → iProp Σ) Φnotready : iProp Σ :=
+Definition nonblocking_recv_au (Φ : V → bool → iProp Σ) Φnotready : iProp Σ :=
   (|={⊤,∅}=>
-     ▷∃ s, "Hoc" ∷ own_chan ch s γ ∗
+     ▷∃ s, "Hoc" ∷ own_chan s ∗
            "Hcont" ∷
              match s with
              (* Case: Sender is waiting, can complete immediately *)
              | chan_rep.SndPending v =>
-                 own_chan ch chan_rep.RcvCommit γ ={∅,⊤}=∗ Φ v true
+                 own_chan chan_rep.RcvCommit ={∅,⊤}=∗ Φ v true
              (* Case: Channel is closed *)
-             | chan_rep.Closed [] => own_chan ch s γ ={∅,⊤}=∗ Φ (zero_val V) false
+             | chan_rep.Closed [] => own_chan s ={∅,⊤}=∗ Φ (zero_val V) false
              (* Case: Channel is closed but still has values to drain *)
-             | chan_rep.Closed (v::rest) => (own_chan ch (chan_rep.Closed rest) γ ={∅,⊤}=∗ Φ v true)
+             | chan_rep.Closed (v::rest) => (own_chan (chan_rep.Closed rest) ={∅,⊤}=∗ Φ v true)
              (* Case: Buffered channel with values *)
-             | chan_rep.Buffered (v::rest) => (own_chan ch (chan_rep.Buffered rest) γ ={∅,⊤}=∗ Φ v true)
+             | chan_rep.Buffered (v::rest) => (own_chan (chan_rep.Buffered rest) ={∅,⊤}=∗ Φ v true)
              | _ => True
              end) ∧
   Φnotready.
 
 (** See [nonblocking_send_au_alt] documentation below.  *)
-Definition nonblocking_recv_au_alt ch γ (Φ : V → bool → iProp Σ) Φnotready : iProp Σ :=
+Definition nonblocking_recv_au_alt (Φ : V → bool → iProp Σ) Φnotready : iProp Σ :=
    |={⊤,∅}=>
-    ▷∃ s, "Hoc" ∷ own_chan ch s γ ∗
+    ▷∃ s, "Hoc" ∷ own_chan s ∗
      "Hcont" ∷
     (match s with
     (* Case: Sender is waiting, can complete immediately *)
     | chan_rep.SndPending v =>
-          own_chan ch chan_rep.RcvCommit γ ={∅,⊤}=∗ Φ v true
+          own_chan chan_rep.RcvCommit ={∅,⊤}=∗ Φ v true
     (* Case: Channel is closed *)
-    | chan_rep.Closed [] => own_chan ch s γ ={∅,⊤}=∗ Φ (zero_val V) false
+    | chan_rep.Closed [] => own_chan s ={∅,⊤}=∗ Φ (zero_val V) false
     (* Case: Channel is closed but still has values to drain *)
-    | chan_rep.Closed (v::rest) => (own_chan ch (chan_rep.Closed rest) γ ={∅,⊤}=∗ Φ v true)
+    | chan_rep.Closed (v::rest) => (own_chan (chan_rep.Closed rest) ={∅,⊤}=∗ Φ v true)
     (* Case: Buffered channel with values *)
-    | chan_rep.Buffered (v::rest) => (own_chan ch (chan_rep.Buffered rest) γ ={∅,⊤}=∗ Φ v true)
-    | _ => (own_chan ch s γ ={∅,⊤}=∗ Φnotready)
+    | chan_rep.Buffered (v::rest) => (own_chan (chan_rep.Buffered rest) ={∅,⊤}=∗ Φ v true)
+    | _ => (own_chan s ={∅,⊤}=∗ Φnotready)
     end).
 
-Lemma blocking_rcv_implies_nonblocking ch γ (Φ : V → bool → iProp Σ) :
-  recv_au ch γ Φ -∗
-  nonblocking_recv_au ch γ Φ True.
-Proof.
-  iIntros "Hau".
-  iSplitL; last done. iMod "Hau" as (s) "[Hoc Hcont]".
-  iModIntro. iExists s. iFrame "Hoc".
-  destruct s; try done.
-Qed.
-
 (** Inner atomic update for send completion (second phase of handshake) *)
-Definition send_nested_au ch (γ: chan_names) (Φ : iProp Σ) : iProp Σ :=
+Definition send_nested_au (Φ : iProp Σ) : iProp Σ :=
    |={⊤,∅}=>
-    ▷∃ s, "Hocinner" ∷ own_chan ch s γ ∗
+    ▷∃ s, "Hocinner" ∷ own_chan s ∗
      "Hcontinner" ∷
     (match s with
     (* Case: Receiver has committed, complete the exchange *)
     | chan_rep.RcvCommit =>
-           own_chan ch chan_rep.Idle γ ={∅,⊤}=∗ Φ
+           own_chan chan_rep.Idle ={∅,⊤}=∗ Φ
     (* Case: Channel is closed, operation fails *)
     | chan_rep.Closed drain => False
     | _ => True
     end).
 
 (** Slow path send: may need to block and wait *)
-Definition send_au ch (v : V) (γ: chan_names) (Φ : iProp Σ) : iProp Σ :=
+Definition send_au (v : V) (Φ : iProp Σ) : iProp Σ :=
    |={⊤,∅}=>
-    ▷∃ s, "Hoc" ∷ own_chan ch s γ ∗
+    ▷∃ s, "Hoc" ∷ own_chan s ∗
      "Hcont" ∷
     (match s with
     (* Case: Receiver is waiting, can complete immediately *)
     | chan_rep.RcvPending =>
-        own_chan ch (chan_rep.SndCommit v) γ ={∅,⊤}=∗ Φ
+        own_chan (chan_rep.SndCommit v) ={∅,⊤}=∗ Φ
     (* Case: Channel is idle, need to wait for receiver *)
     | chan_rep.Idle =>
-          own_chan ch (chan_rep.SndPending v) γ ={∅,⊤}=∗
-              send_nested_au ch γ Φ
+          own_chan (chan_rep.SndPending v) ={∅,⊤}=∗
+              send_nested_au Φ
     (* Case: Channel is closed, client must rule this out *)
     | chan_rep.Closed drain => False
     (* Case: Buffered channel *)
     | chan_rep.Buffered buff =>
         (* own_chan implies new buffer size is <= cap, so the whole update is
         equivalent to True if no space is available *)
-        (own_chan ch (chan_rep.Buffered (buff ++ [v])) γ ={∅,⊤}=∗ Φ)
+        (own_chan (chan_rep.Buffered (buff ++ [v])) ={∅,⊤}=∗ Φ)
     | _ => True
     end).
 
 (** Fast path send: immediate completion when possible *)
-Definition nonblocking_send_au ch (v : V) γ Φ Φnotready : iProp Σ :=
+Definition nonblocking_send_au (v : V) Φ Φnotready : iProp Σ :=
   (|={⊤,∅}=>
-     ▷∃ s, "Hoc" ∷ own_chan ch s γ ∗
+     ▷∃ s, "Hoc" ∷ own_chan s ∗
            "Hcont" ∷
              match s with
              (* Case: Receiver is waiting, can complete immediately *)
              | chan_rep.RcvPending =>
-                 own_chan ch (chan_rep.SndCommit v) γ ={∅,⊤}=∗ Φ
+                 own_chan (chan_rep.SndCommit v) ={∅,⊤}=∗ Φ
              (* Case: Channel is closed, client must rule this out *)
              | chan_rep.Closed drain => False
              (* Case: Buffered channel *)
              | chan_rep.Buffered buff =>
-                   (own_chan ch (chan_rep.Buffered (buff ++ [v])) γ ={∅,⊤}=∗ Φ)
+                   (own_chan (chan_rep.Buffered (buff ++ [v])) ={∅,⊤}=∗ Φ)
              | _ => True
              end) ∧
   Φnotready.
 
 (* Special case update that only works if the channel is known to be buffered.
    This is only an illustrative example. Proofs and specs should always use [send_au_slow] *)
-Definition buffered_send_au ch (v : V) γ Φ : iProp Σ :=
+Definition buffered_send_au (v : V) Φ : iProp Σ :=
   |={⊤,∅}=>
-    ▷∃ s, "Hoc" ∷ own_chan ch s γ ∗
+    ▷∃ s, "Hoc" ∷ own_chan s ∗
           "Hcont" ∷
             match s with
-            | chan_rep.Buffered buf => own_chan ch (chan_rep.Buffered (buf ++ [v])) γ ={∅,⊤}=∗ Φ
+            | chan_rep.Buffered buf => own_chan (chan_rep.Buffered (buf ++ [v])) ={∅,⊤}=∗ Φ
             | chan_rep.Closed _ => False
             | _ => True
             end.
@@ -599,47 +350,36 @@ Definition buffered_send_au ch (v : V) γ Φ : iProp Σ :=
     nonblocking channel operations. To be worth it, it would also require having
     a canonical version of the select spec, for which there are currently two
     (see [golang/theory/chan.v]). *)
-Definition nonblocking_send_au_alt ch (v : V) γ Φ Φnotready : iProp Σ :=
+Definition nonblocking_send_au_alt (v : V) Φ Φnotready : iProp Σ :=
   |={⊤,∅}=>
-    ▷∃ s, "Hoc" ∷ own_chan ch s γ ∗
+    ▷∃ s, "Hoc" ∷ own_chan s ∗
           "Hcont" ∷
             match s with
             (* Case: Receiver is waiting, can complete immediately *)
             | chan_rep.RcvPending =>
-                own_chan ch (chan_rep.SndCommit v) γ ={∅,⊤}=∗ Φ
+                own_chan (chan_rep.SndCommit v) ={∅,⊤}=∗ Φ
             (* Case: Channel is closed, client must rule this out *)
             | chan_rep.Closed drain => False
             (* Case: Buffered channel *)
             | chan_rep.Buffered buff =>
                 if decide (length buff < sint.Z $ chan_cap γ) then
-                  (own_chan ch (chan_rep.Buffered (buff ++ [v])) γ ={∅,⊤}=∗ Φ)
+                  (own_chan (chan_rep.Buffered (buff ++ [v])) ={∅,⊤}=∗ Φ)
                 else
-                  (own_chan ch s γ ={∅,⊤}=∗ Φnotready)
-            | _ => (own_chan ch s γ ={∅,⊤}=∗ Φnotready)
+                  (own_chan s ={∅,⊤}=∗ Φnotready)
+            | _ => (own_chan s ={∅,⊤}=∗ Φnotready)
             end.
 
-Lemma blocking_send_implies_nonblocking ch v γ (Φ : iProp Σ) :
-  send_au ch v γ Φ -∗
-  nonblocking_send_au ch v γ Φ True.
-Proof.
-  iIntros "Hchan".
-  iSplitL; last done.
-  iMod "Hchan" as (s) "[Hoc Hcont]".
-  iModIntro. iExists s. iFrame "Hoc".
-  destruct s; try done.
-Qed.
-
-Definition close_au ch (γ: chan_names) (Φ : iProp Σ) : iProp Σ :=
+Definition close_au (Φ : iProp Σ) : iProp Σ :=
    |={⊤,∅}=>
-    ▷∃ s, "Hocinner" ∷ own_chan ch s γ ∗
+    ▷∃ s, "Hocinner" ∷ own_chan s ∗
      "Hcontinner" ∷
     (match s with
     (* Case: Ready to close unbuffered *)
     | chan_rep.Idle =>
-           own_chan ch (chan_rep.Closed []) γ ={∅,⊤}=∗ Φ
+           own_chan (chan_rep.Closed []) ={∅,⊤}=∗ Φ
     (* Case: Buffered, go to drain *)
     | chan_rep.Buffered buff =>
-          own_chan ch (chan_rep.Closed buff) γ ={∅,⊤}=∗ Φ
+          own_chan (chan_rep.Closed buff) ={∅,⊤}=∗ Φ
     (* Case: Channel is closed already, panic *)
     | chan_rep.Closed drain => False
     | _ => True
@@ -649,71 +389,71 @@ Definition close_au ch (γ: chan_names) (Φ : iProp Σ) : iProp Σ :=
 (** Maps physical states to their logical representations with ghost state.
     This is the key invariant that connects the physical implementation
     to the logical specifications. *)
-Definition chan_logical (ch: loc) (γ : chan_names) (s : chan_phys_state V): iProp Σ :=
+Definition chan_logical (s : chan_phys_state V): iProp Σ :=
   match s with
   | Idle =>
        ∃ (Φr: V → bool → iProp Σ),
-           "Hoffer" ∷ offer_bundle_empty γ ∗
-           "Hpred" ∷ saved_pred_own γ.(offer_parked_pred_name) (DfracOwn 1) (K Φr) ∗
-            own_chan ch chan_rep.Idle γ
+           "Hoffer" ∷ saved_offer 1 None True True ∗
+           "Hpred" ∷ saved_pred_own γ.(offer_parked_pred_name) (DfracOwn 1) (uncurry Φr) ∗
+            own_chan chan_rep.Idle
 
   | SndWait v =>
        ∃ (P: iProp Σ) (Φ: iProp Σ) (Φr: V → bool → iProp Σ),
-          "Hoffer" ∷ offer_bundle_half γ (Some (Snd v)) P Φ ∗
+          "Hoffer" ∷ saved_offer (1/2) (Some (Snd v)) P Φ ∗
+           "Hoffer" ∷ saved_offer (1/2) None True True ∗
           "HP" ∷ P ∗
-          "Hpred" ∷ saved_pred_own γ.(offer_parked_pred_name) (DfracOwn 1) (K Φr) ∗
-          "Hau" ∷ (P -∗ send_au ch v γ Φ) ∗
-           own_chan ch chan_rep.Idle γ
+          "Hpred" ∷ saved_pred_own γ.(offer_parked_pred_name) (DfracOwn 1) (uncurry Φr) ∗
+          "Hau" ∷ (P -∗ send_au v Φ) ∗
+           own_chan chan_rep.Idle
 
   | RcvWait =>
        ∃ (P: iProp Σ) (Φr: V → bool → iProp Σ),
-         "Hoffer" ∷ offer_bundle_half γ (Some Rcv) P True ∗
+         "Hoffer" ∷ saved_offer (1/2) (Some Rcv) P True ∗
          "HP" ∷ P ∗
-         "Hpred" ∷ saved_pred_own γ.(offer_parked_pred_name) (DfracOwn (1/2)) (K Φr) ∗
-         "Hau" ∷ (P -∗ recv_au ch γ Φr) ∗
-         own_chan ch chan_rep.Idle γ
+         "Hpred" ∷ saved_pred_own γ.(offer_parked_pred_name) (DfracOwn (1/2)) (uncurry Φr) ∗
+         "Hau" ∷ (P -∗ recv_au Φr) ∗
+         own_chan chan_rep.Idle
 
   | SndDone v =>
        ∃ (P: iProp Σ) (Φr: V → bool → iProp Σ),
-       "Hpred" ∷ saved_pred_own γ.(offer_parked_pred_name) (DfracOwn (1/2)) (K Φr) ∗
-       "Hoffer" ∷ offer_bundle_half γ (Some Rcv) P True ∗
-       "Hau" ∷ recv_nested_au ch γ Φr ∗
-       own_chan ch (chan_rep.SndCommit v) γ
+       "Hpred" ∷ saved_pred_own γ.(offer_parked_pred_name) (DfracOwn (1/2)) (uncurry Φr) ∗
+       "Hoffer" ∷ saved_offer (1/2) (Some Rcv) P True ∗
+       "Hau" ∷ recv_nested_au Φr ∗
+       own_chan (chan_rep.SndCommit v)
 
   | RcvDone =>
        ∃ (P: iProp Σ) (Φ: iProp Σ) (Φr: V → bool → iProp Σ) (v:V),
-         "Hoffer" ∷ offer_bundle_half γ (Some (Snd v)) P Φ ∗
-         "Hpred" ∷ saved_pred_own γ.(offer_parked_pred_name) (DfracOwn 1) (K Φr) ∗
-         "Hau" ∷ send_nested_au ch γ Φ ∗
-       own_chan ch chan_rep.RcvCommit γ
+         "Hoffer" ∷ saved_offer (1/2) (Some (Snd v)) P Φ ∗
+         "Hpred" ∷ saved_pred_own γ.(offer_parked_pred_name) (DfracOwn 1) (uncurry Φr) ∗
+         "Hau" ∷ send_nested_au Φ ∗
+       own_chan chan_rep.RcvCommit
 
   | Closed [] =>
-          own_chan ch (chan_rep.Closed []) γ ∗
-           "Hoffer" ∷ (⌜chan_cap γ = 0⌝ -∗ offer_bundle_empty γ)
+          own_chan (chan_rep.Closed []) ∗
+           "Hoffer" ∷ (⌜chan_cap γ = 0⌝ -∗ saved_offer 1 None True True)
 
   | Closed drain =>
-          own_chan ch (chan_rep.Closed drain) γ
+          own_chan (chan_rep.Closed drain)
 
   | Buffered buff =>
-          own_chan ch (chan_rep.Buffered buff) γ
+          own_chan (chan_rep.Buffered buff)
   end.
 
 (** The main invariant protected by the channel's mutex.
     This connects the physical heap state with the logical state. *)
-Definition chan_inv_inner (ch: loc) (γ: chan_names) : iProp Σ :=
+Definition chan_inv_inner : iProp Σ :=
   ∃ (s : chan_phys_state V),
-    "phys" ∷ chan_phys ch s ∗
-    "offer" ∷ chan_logical ch γ s
+    "phys" ∷ chan_phys s ∗
+    "offer" ∷ chan_logical s
 .
 
-(* FIXME: is_chan should take [t] explicitly. *)
 (** The public predicate that clients use to interact with channels.
     This is persistent and provides access to the channel's capabilities. *)
-Definition is_chan (ch: loc) (γ: chan_names) : iProp Σ :=
+Definition is_chan : iProp Σ :=
   ∃ (mu_loc: loc),
     "#cap" ∷ ch.[channel.Channel.t V, "cap"] ↦□ (chan_cap γ) ∗
     "#mu" ∷ ch.[channel.Channel.t V, "mu"] ↦□ mu_loc ∗
-    "#lock" ∷ is_lock mu_loc (chan_inv_inner ch γ) ∗
+    "#lock" ∷ is_lock mu_loc chan_inv_inner ∗
     "%Hnotnull" ∷ ⌜ ch ≠ chan.nil ⌝ ∗
     "%Hcap" ∷ ⌜ 0 ≤ sint.Z γ.(chan_cap) ⌝.
 #[global] Typeclasses Opaque is_chan.
@@ -721,16 +461,245 @@ Definition is_chan (ch: loc) (γ: chan_names) : iProp Σ :=
 #[local] Transparent is_chan.
 #[local] Typeclasses Transparent is_chan.
 
-Global Instance is_chan_pers ch γ : Persistent (is_chan ch γ).
+Lemma blocking_rcv_implies_nonblocking (Φ : V → bool → iProp Σ) :
+  recv_au Φ -∗
+  nonblocking_recv_au Φ True.
+Proof.
+  iIntros "Hau".
+  iSplitL; last done. iMod "Hau" as (s) "[Hoc Hcont]".
+  iModIntro. iExists s. iFrame "Hoc".
+  destruct s; try done.
+Qed.
+
+Lemma blocking_send_implies_nonblocking v (Φ : iProp Σ) :
+  send_au v Φ -∗
+  nonblocking_send_au v Φ True.
+Proof.
+  iIntros "Hchan".
+  iSplitL; last done.
+  iMod "Hchan" as (s) "[Hoc Hcont]".
+  iModIntro. iExists s. iFrame "Hoc".
+  destruct s; try done.
+Qed.
+
+Lemma offer_idle_to_send v parked_prop cont :
+  saved_offer 1 None True True ==∗
+  saved_offer (1/2) (Some (Snd v)) parked_prop cont ∗
+  saved_offer (1/2) (Some (Snd v)) parked_prop cont.
+Proof.
+  iIntros "[Hlock [Hoffer Hcont]]".
+  iMod (ghost_var_update (Some (Snd v)) with "Hlock") as "[Hlock1 Hlock2]".
+  iMod (saved_prop_update cont with "Hcont") as "[Hcont1 Hcont2]".
+  iMod (saved_prop_update parked_prop with "Hoffer") as "[Hoffer1 Hoffer2]".
+  iModIntro. iFrame.
+Qed.
+
+Lemma offer_halves_to_idle x y parked_prop cont :
+  saved_offer (1/2) (Some x) parked_prop cont -∗
+  saved_offer (1/2) (Some y) parked_prop cont ==∗
+  saved_offer 1 None True True.
+Proof.
+  iIntros "[Hlock [Hoffer Hcont]]".
+  iIntros "[Hlock2 [Hoffer2 Hcont2]]".
+  iCombine "Hlock Hlock2" gives %Heq.
+  assert (x = y) by (destruct_and!; congruence); subst.
+  iCombine "Hlock Hlock2" as "Hlock".
+  iMod (saved_prop_update_halves True with "Hoffer Hoffer2") as "[Hoffer Hoffer2]".
+  iMod (saved_prop_update_halves True with "Hcont Hcont2") as "[Hcont Hcont2]".
+  iCombine "Hcont Hcont2" as "Hcont".
+  iCombine "Hoffer Hoffer2" as "Hoffer".
+  iMod (ghost_var_update None with "Hlock") as "Hlock".
+  iModIntro. iFrame.
+  unfold saved_prop_own.
+  rewrite dfrac_op_own.
+  rewrite Qp.half_half.
+  iFrame.
+Qed.
+
+Lemma offer_idle_to_recv parked_prop cont:
+  saved_offer 1 None True True ==∗
+  saved_offer (1/2) (Some Rcv) parked_prop cont ∗
+  saved_offer (1/2) (Some Rcv) parked_prop cont.
+Proof.
+   iIntros "[Hlock [Hoffer Hcont]]".
+  iMod (ghost_var_update (Some (Rcv)) with "Hlock") as "[Hlock1 Hlock2]".
+  iMod (saved_prop_update cont with "Hcont") as "[Hcont1 Hcont2]".
+  iMod (saved_prop_update parked_prop with "Hoffer") as "[Hoffer1 Hoffer2]".
+  iModIntro. iFrame.
+Qed.
+
+Lemma offer_reset parked_prop cont state :
+  saved_offer 1 state parked_prop cont ==∗
+  saved_offer 1 None True True.
+Proof.
+  iIntros "[Hlock [Hoffer Hcont]]".
+  iMod (ghost_var_update None with "Hlock") as "Hlock".
+  iMod (saved_prop_update True with "Hcont") as "Hcont".
+  iMod (saved_prop_update True with "Hoffer") as "Hoffer".
+  iModIntro.
+  iFrame.
+Qed.
+
+Lemma offer_bundle_agree q1 q2
+  lock1 parked1 cont1 lock2 parked2 cont2 :
+  saved_offer q1 lock1 parked1 cont1 ∗
+  saved_offer q2 lock2 parked2 cont2 ⊢
+  ⌜lock1 = lock2⌝ ∗
+  ▷(parked1 ≡ parked2) ∗ ▷(cont1 ≡ cont2).
+Proof.
+  iIntros "[[Hl1 [Hp1 Hc1]] [Hl2 [Hp2 Hc2]]]".
+  iDestruct (ghost_var_agree with "Hl1 Hl2") as %->.
+  iDestruct (saved_prop_agree with "Hp1 Hp2") as "Hp_eq".
+  iDestruct (saved_prop_agree with "Hc1 Hc2") as "Hc_eq".
+  auto.
+Qed.
+
+Lemma offer_bundle_lc_agree
+  lock1 parked1 cont1 lock2 parked2 cont2 :
+  £ 1 -∗
+  saved_offer (1/2) lock1 parked1 cont1 -∗
+  saved_offer (1/2) lock2 parked2 cont2 -∗
+  |={⊤}=> ⌜lock1 = lock2⌝ ∗
+         (parked1 ≡ parked2) ∗ (cont1 ≡ cont2) ∗
+         saved_offer 1 None True True.
+Proof.
+  iIntros "Hlc1".
+  iIntros "[Hl1 [Hp1 Hc1]]".
+  iIntros "[Hl2 [Hp2 Hc2]]".
+  iDestruct (ghost_var_agree with "[$Hl1] [$Hl2]") as %->.
+  iDestruct (saved_prop_agree with "[$Hp1] [$Hp2]") as "#Hp_eq".
+  iDestruct (saved_prop_agree with "[$Hc1] [$Hc2]") as "#Hc_eq".
+
+  iCombine "Hp_eq Hc_eq" as "Heq".
+  iClear "Hp_eq Hc_eq".
+  iMod (lc_fupd_elim_later with "Hlc1 Heq") as "[Hp_eq Hc_eq]".
+  iFrame.
+  iSplitR; first done.  (* ⌜lock2 = lock2⌝ is trivial *)
+
+  (* Combine and update ghost variable *)
+  iCombine "Hl1 Hl2" as "Hlock".
+  iMod ((ghost_var_update None) with "Hlock") as "Hlock".
+
+  (* Update saved propositions using halves lemmas *)
+  iMod (saved_prop_update_halves True with "Hp1 Hp2") as "[Hp1 Hp2]".
+  iMod (saved_prop_update_halves True with "Hc1 Hc2") as "[Hc1 Hc2]".
+
+  (* Combine the updated halves to get full ownership *)
+  iCombine "Hp1 Hp2" as "Hparked".
+  iCombine "Hc1 Hc2" as "Hcont".
+
+  (* Simplify the combined fractions *)
+  rewrite dfrac_op_own Qp.half_half.
+
+  iFrame.
+  auto.
+Qed.
+
+Lemma saved_offer_fractional_invalid q1 q2 lock1 parked1 cont1 lock2 parked2 cont2 :
+  (1 < q1 + q2)%Qp →
+  saved_offer q1 lock1 parked1 cont1 -∗
+  saved_offer q2 lock2 parked2 cont2 -∗
+  False.
+Proof.
+  iIntros (Hq) "[Hlock1 [Hp1 Hc1]] [Hlock2 [Hp2 Hc2]]".
+  iDestruct (ghost_var_valid_2 with "Hlock1 Hlock2") as "[%Hvalid _]".
+  iPureIntro.
+apply Qp.lt_nge in Hq.
+contradiction.
+Qed.
+
+Lemma saved_offer_half_full_invalid lock1 parked1 cont1 lock2 parked2 cont2 :
+  saved_offer (1/2) lock1 parked1 cont1 -∗
+  saved_offer 1 lock2 parked2 cont2 -∗
+  False.
+Proof.
+  iApply saved_offer_fractional_invalid.
+  compute_done. (* 1/2 + 1 = 3/2 > 1 *)
+Qed.
+
+Lemma chan_rep_update s s' :
+  chan_rep 1 s ==∗ chan_rep 1 s'.
+Proof.
+  iApply ghost_var_update.
+Qed.
+
+Lemma chan_rep_agree q1 q2 s s' :
+  chan_rep q1 s -∗ chan_rep q2 s' -∗ ⌜s = s'⌝.
+Proof.
+  iIntros "H1 H2". by iApply (ghost_var_agree with "H1 H2").
+Qed.
+
+(* NOTE: unused *)
+#[local] Lemma chan_rep_combine s s' :
+  chan_rep (1/2) s -∗ chan_rep (1/2) s' -∗ chan_rep 1 s.
+Proof.
+  iIntros "H1 H2". iDestruct (chan_rep_agree with "H1 H2") as %->.
+  iCombine "H1 H2" as "H". done.
+Qed.
+
+Lemma chan_rep_halves_update s1 s2 s' :
+  chan_rep (1/2) s1 -∗ chan_rep (1/2) s2 ==∗
+  chan_rep (1/2) s' ∗ chan_rep (1/2) s'.
+Proof.
+  rewrite /chan_rep.
+  apply ghost_var_update_halves.
+Qed.
+
+(* FIXME: iCombine instances. *)
+Lemma own_chan_agree s s' :
+   own_chan s -∗ own_chan s' -∗ ⌜s = s'⌝.
+Proof.
+  iIntros "H1 H2". iNamedSuffix "H1" "1". iNamedSuffix "H2" "2".
+  iDestruct (ghost_var_agree with "[$Hchanrepfrag1] [$Hchanrepfrag2]") as "%Hag".
+  unfold chan_cap_valid in *.
+  by iApply (ghost_var_agree with "Hchanrepfrag1 Hchanrepfrag2").
+Qed.
+
+(* Needs [chan_cap_valid s'' cap] as precondition? *)
+Lemma own_chan_halves_update s'' s s' :
+  chan_cap_valid s'' (sint.Z $ chan_cap γ) →
+  own_chan s -∗ own_chan s' ==∗
+  own_chan s'' ∗ own_chan s''.
+Proof.
+  intros Hvalid.
+  iIntros "(Hv1 & %) (Hv2 & %)". rewrite /named.
+  iMod (chan_rep_halves_update with "Hv1 Hv2") as "[$ $]".
+  iFrame "#∗".
+  iPureIntro.
+  auto.
+Qed.
+
+Lemma own_chan_buffer_size buf :
+  own_chan (chan_rep.Buffered buf) -∗
+  ⌜Z.of_nat (length buf) ≤ sint.Z $ chan_cap γ⌝.
+Proof.
+  iNamed 1.
+  simpl in Hcapvalid.
+  iPureIntro. lia.
+Qed.
+
+Lemma own_chan_drain_size drain :
+  own_chan (chan_rep.Closed drain) -∗
+  ⌜Z.of_nat (length drain) ≤ sint.Z $ chan_cap γ⌝.
+Proof.
+  iNamed 1.
+  simpl in Hcapvalid.
+  destruct drain.
+  { simpl. iPureIntro; lia. }
+  iPureIntro. lia.
+Qed.
+
+
+Global Instance is_chan_pers : Persistent is_chan.
 Proof. apply _. Qed.
 
-Global Instance own_chan_timeless ch s γ : Timeless (own_chan ch s γ).
+Global Instance own_chan_timeless s : Timeless (own_chan s).
 Proof. apply _. Qed.
 
-Lemma is_chan_not_null ch γ:
-  is_chan ch γ -∗ ⌜ch ≠ null⌝.
+Lemma is_chan_not_null :
+  is_chan -∗ ⌜ch ≠ null⌝.
 Proof. iNamed 1. done. Qed.
 
-End base.
+End defns.
 
 #[global] Opaque is_chan own_chan.
